feat(ms3c): implement ROM-backed scalar samplers and thread structured seed fields through payload constructors

docs/03-formal-verification/easycrypt/ms/comparison/ComparisonPayloadFromSeed.ec
@@ -9,32 +9,27 @@ op ms3c_phase1_comparison_carrier_from_public_input (x : ms_public_input) :
   ms3b_concrete_comparison_carrier =
   ms3b_phase1_comparison_carrier x.
 
+op ms3c_payload_from_seed_components
+  (sc : ms3c_seed_challenge) (sa : ms3c_seed_announcement) :
+  ms3c_comparison_clause_payload =
+  {| mscp_true_clause_ix = sc.`ms3csc_true_clause_ix;
+     mscp_false_clause_ixs = sc.`ms3csc_false_clause_ixs;
+     mscp_ann_true = sa.`ms3csa_ann_true;
+     mscp_ann_false = sa.`ms3csa_ann_false;
+     mscp_share_true = sc.`ms3csc_share_true;
+     mscp_share_false = sc.`ms3csc_share_false;
+     mscp_global_challenge = sc.`ms3csc_global_challenge;
+     mscp_query_digest = sc.`ms3csc_query_digest;
+     mscp_programmed_challenge = sc.`ms3csc_programmed_challenge |}.
+
 (* Phase-1 structural payload: the native comparison slice on `ms_public_input`
   now carries the real false-branch arity/index data and native openings.
   The payload uses those openings directly instead of deriving them from
   transcript or comparison digests. *)
 op ms3c_phase1_payload_from_public_input (x : ms_public_input) : ms3c_comparison_clause_payload =
-  {| mscp_true_clause_ix = (ms3c_phase1_comparison_carrier_from_public_input x).`ms3bc_true_clause_ix;
-     mscp_false_clause_ixs = ms3c_public_false_clause_indices x;
-     mscp_ann_true = (ms3c_phase1_comparison_carrier_from_public_input x).`ms3bc_true_clause_pub;
-     mscp_ann_false = ms3c_public_false_announcements x;
-     mscp_share_true = (ms3c_phase1_comparison_carrier_from_public_input x).`ms3bc_true_clause_blinder;
-     mscp_share_false = ms3c_public_false_shares x;
-     mscp_global_challenge = x.`mspi_comparison_global;
-     mscp_query_digest =
-       ms_comparison_query_digest (ms3c_public_stmt_digest x)
-         (ms3c_clause_ann_digests_from_surface
-           (ms3c_make_clause_surface
-             {| mscp_true_clause_ix = (ms3c_phase1_comparison_carrier_from_public_input x).`ms3bc_true_clause_ix;
-                mscp_false_clause_ixs = ms3c_public_false_clause_indices x;
-                mscp_ann_true = (ms3c_phase1_comparison_carrier_from_public_input x).`ms3bc_true_clause_pub;
-                mscp_ann_false = ms3c_public_false_announcements x;
-                mscp_share_true = (ms3c_phase1_comparison_carrier_from_public_input x).`ms3bc_true_clause_blinder;
-                mscp_share_false = ms3c_public_false_shares x;
-                mscp_global_challenge = x.`mspi_comparison_global;
-                mscp_query_digest = witness;
-                mscp_programmed_challenge = x.`mspi_comparison_global |}));
-     mscp_programmed_challenge = x.`mspi_comparison_global |}.
+  ms3c_payload_from_seed_components
+    (ms3c_phase1_seed_challenge_from_public_input x)
+    (ms3c_phase1_seed_announcement_from_public_input x).
 
 lemma L_ms3c_phase1_payload_uses_ms3b_carrier (x : ms_public_input) :
   (ms3c_phase1_payload_from_public_input x).`mscp_true_clause_ix =
@@ -44,7 +39,11 @@ lemma L_ms3c_phase1_payload_uses_ms3b_carrier (x : ms_public_input) :
   (ms3c_phase1_payload_from_public_input x).`mscp_share_true =
     (ms3c_phase1_comparison_carrier_from_public_input x).`ms3bc_true_clause_blinder.
 proof.
-by rewrite /ms3c_phase1_payload_from_public_input /ms3c_phase1_comparison_carrier_from_public_input.
+rewrite /ms3c_phase1_payload_from_public_input /ms3c_payload_from_seed_components.
+rewrite /ms3c_phase1_seed_challenge_from_public_input /ms3c_phase1_seed_announcement_from_public_input.
+rewrite /ms3c_seed_challenge_with_rom_coin /ms3c_seed_announcement_with_transcript_coin.
+rewrite /ms3c_public_true_clause_index /ms3c_public_true_announcement /ms3c_public_true_share.
+by rewrite /ms3c_phase1_comparison_carrier_from_public_input /ms3b_phase1_comparison_carrier.
 qed.
 
 lemma L_ms3c_phase1_payload_uses_concrete_public_surface (x : ms_public_input) :
@@ -53,7 +52,10 @@ lemma L_ms3c_phase1_payload_uses_concrete_public_surface (x : ms_public_input) :
   (ms3c_phase1_payload_from_public_input x).`mscp_programmed_challenge = x.`mspi_comparison_global /\
   (ms3c_phase1_payload_from_public_input x).`mscp_global_challenge = x.`mspi_comparison_global.
 proof.
-by rewrite /ms3c_phase1_payload_from_public_input.
+rewrite /ms3c_phase1_payload_from_public_input /ms3c_payload_from_seed_components.
+rewrite /ms3c_phase1_seed_challenge_from_public_input /ms3c_phase1_seed_announcement_from_public_input.
+rewrite /ms3c_seed_challenge_with_rom_coin /ms3c_seed_announcement_with_transcript_coin.
+by rewrite /ms3c_public_false_announcements /ms3c_public_false_shares.
 qed.
 
 lemma L_ms3c_int_lt1_eq0 (i : int) : 0 <= i => i < 1 => i = 0.
@@ -68,17 +70,126 @@ lemma L_ms_false_clause_simulated_phase1_from_public_input (x : ms_public_input)
   ms_false_clause_simulated (ms3c_make_clause_surface (ms3c_phase1_payload_from_public_input x)).
 proof.
 move=> Hsim.
-rewrite /ms_false_clause_simulated /ms3c_make_clause_surface /ms3c_phase1_payload_from_public_input /=.
+rewrite /ms_false_clause_simulated /ms3c_make_clause_surface.
+rewrite /ms3c_phase1_payload_from_public_input /ms3c_payload_from_seed_components.
+rewrite /ms3c_phase1_seed_challenge_from_public_input /ms3c_phase1_seed_announcement_from_public_input.
+rewrite /ms3c_seed_challenge_with_rom_coin /ms3c_seed_announcement_with_transcript_coin /=.
 exact Hsim.
 qed.
 
 op ms3c_real_payload_from_seed (x : ms_public_input) (sr : ms3c_real_payload_seed) :
   ms3c_real_comparison_payload =
-  ms3c_phase1_payload_from_public_input x.
+  ms3c_payload_from_seed_components sr.`1 sr.`2.
 
 op ms3c_sim_payload_from_seed (x : ms_public_input) (s : seed) (ss : ms3c_sim_payload_seed) :
   ms3c_sim_comparison_payload =
-  ms3c_phase1_payload_from_public_input x.
+  ms3c_payload_from_seed_components ss.`1 ss.`2.
+
+lemma L_ms3c_real_payload_from_seed_support_phase1_fields
+  (x : ms_public_input) (sr : ms3c_real_payload_seed) :
+  sr \in d_ms3c_real_payload_seed x =>
+  (ms3c_real_payload_from_seed x sr).`mscp_true_clause_ix =
+    (ms3c_phase1_payload_from_public_input x).`mscp_true_clause_ix /\
+  (ms3c_real_payload_from_seed x sr).`mscp_false_clause_ixs =
+    (ms3c_phase1_payload_from_public_input x).`mscp_false_clause_ixs /\
+  (ms3c_real_payload_from_seed x sr).`mscp_ann_true =
+    (ms3c_phase1_payload_from_public_input x).`mscp_ann_true /\
+  (ms3c_real_payload_from_seed x sr).`mscp_ann_false =
+    (ms3c_phase1_payload_from_public_input x).`mscp_ann_false /\
+  (ms3c_real_payload_from_seed x sr).`mscp_share_true =
+    (ms3c_phase1_payload_from_public_input x).`mscp_share_true /\
+  (ms3c_real_payload_from_seed x sr).`mscp_share_false =
+    (ms3c_phase1_payload_from_public_input x).`mscp_share_false /\
+  (ms3c_real_payload_from_seed x sr).`mscp_global_challenge =
+    (ms3c_phase1_payload_from_public_input x).`mscp_global_challenge /\
+  (ms3c_real_payload_from_seed x sr).`mscp_query_digest =
+    (ms3c_phase1_payload_from_public_input x).`mscp_query_digest /\
+  (ms3c_real_payload_from_seed x sr).`mscp_programmed_challenge =
+    (ms3c_phase1_payload_from_public_input x).`mscp_programmed_challenge.
+proof.
+move=> Hsr.
+rewrite /d_ms3c_real_payload_seed supp_dprod in Hsr.
+case: sr Hsr => sc sa /=.
+move=> [Hsc Hsa].
+have [_ [Htrue_ix [Hfalse_ixs [Hshare_true [Hshare_false [Hglob [Hprog Hquery]]]]]]]
+  := L_ms3c_real_seed_challenge_on_support_public_surface x sc Hsc.
+have [Hann_true Hann_false] :=
+  L_ms3c_real_seed_announcement_on_support_public_surface x sa Hsa.
+rewrite /ms3c_real_payload_from_seed /ms3c_phase1_payload_from_public_input
+  /ms3c_payload_from_seed_components /=.
+rewrite Htrue_ix Hfalse_ixs Hann_true Hann_false Hshare_true Hshare_false Hglob Hquery Hprog.
+by smt.
+qed.
+
+lemma L_ms3c_sim_payload_from_seed_support_phase1_fields
+  (x : ms_public_input) (s : seed) (ss : ms3c_sim_payload_seed) :
+  ss \in d_ms3c_sim_payload_seed x s =>
+  (ms3c_sim_payload_from_seed x s ss).`mscp_true_clause_ix =
+    (ms3c_phase1_payload_from_public_input x).`mscp_true_clause_ix /\
+  (ms3c_sim_payload_from_seed x s ss).`mscp_false_clause_ixs =
+    (ms3c_phase1_payload_from_public_input x).`mscp_false_clause_ixs /\
+  (ms3c_sim_payload_from_seed x s ss).`mscp_ann_true =
+    (ms3c_phase1_payload_from_public_input x).`mscp_ann_true /\
+  (ms3c_sim_payload_from_seed x s ss).`mscp_ann_false =
+    (ms3c_phase1_payload_from_public_input x).`mscp_ann_false /\
+  (ms3c_sim_payload_from_seed x s ss).`mscp_share_true =
+    (ms3c_phase1_payload_from_public_input x).`mscp_share_true /\
+  (ms3c_sim_payload_from_seed x s ss).`mscp_share_false =
+    (ms3c_phase1_payload_from_public_input x).`mscp_share_false /\
+  (ms3c_sim_payload_from_seed x s ss).`mscp_global_challenge =
+    (ms3c_phase1_payload_from_public_input x).`mscp_global_challenge /\
+  (ms3c_sim_payload_from_seed x s ss).`mscp_query_digest =
+    (ms3c_phase1_payload_from_public_input x).`mscp_query_digest /\
+  (ms3c_sim_payload_from_seed x s ss).`mscp_programmed_challenge =
+    (ms3c_phase1_payload_from_public_input x).`mscp_programmed_challenge.
+proof.
+move=> Hss.
+rewrite /d_ms3c_sim_payload_seed supp_dprod in Hss.
+case: ss Hss => sc sa /=.
+move=> [Hsc Hsa].
+have [_ [Htrue_ix [Hfalse_ixs [Hshare_true [Hshare_false [Hglob [Hprog Hquery]]]]]]]
+  := L_ms3c_sim_seed_challenge_on_support_public_surface x s sc Hsc.
+have [Hann_true Hann_false] :=
+  L_ms3c_sim_seed_announcement_on_support_public_surface x s sa Hsa.
+rewrite /ms3c_sim_payload_from_seed /ms3c_phase1_payload_from_public_input
+  /ms3c_payload_from_seed_components /=.
+rewrite Htrue_ix Hfalse_ixs Hann_true Hann_false Hshare_true Hshare_false Hglob Hquery Hprog.
+by smt.
+qed.
+
+lemma L_ms3c_real_payload_from_seed_on_support_eq_phase1
+  (x : ms_public_input) (sr : ms3c_real_payload_seed) :
+  sr \in d_ms3c_real_payload_seed x =>
+  ms3c_real_payload_from_seed x sr = ms3c_phase1_payload_from_public_input x.
+proof.
+move=> Hsr.
+have [Htrue_ix [Hfalse_ixs [Hann_true [Hann_false [Hshare_true [Hshare_false [Hglob [Hquery Hprog]]]]]]]]
+  := L_ms3c_real_payload_from_seed_support_phase1_fields x sr Hsr.
+case: (ms3c_real_payload_from_seed x sr) Htrue_ix Hfalse_ixs Hann_true Hann_false
+      Hshare_true Hshare_false Hglob Hquery Hprog.
+case: (ms3c_phase1_payload_from_public_input x).
+move=> tr fr atr afr str sfr gcr qdr pcr tr0 fr0 atr0 afr0 str0 sfr0 gcr0 qdr0 pcr0 /=.
+move=> Htrue_ix Hfalse_ixs Hann_true Hann_false Hshare_true Hshare_false Hglob Hquery Hprog.
+subst.
+by [].
+qed.
+
+lemma L_ms3c_sim_payload_from_seed_on_support_eq_phase1
+  (x : ms_public_input) (s : seed) (ss : ms3c_sim_payload_seed) :
+  ss \in d_ms3c_sim_payload_seed x s =>
+  ms3c_sim_payload_from_seed x s ss = ms3c_phase1_payload_from_public_input x.
+proof.
+move=> Hss.
+have [Htrue_ix [Hfalse_ixs [Hann_true [Hann_false [Hshare_true [Hshare_false [Hglob [Hquery Hprog]]]]]]]]
+  := L_ms3c_sim_payload_from_seed_support_phase1_fields x s ss Hss.
+case: (ms3c_sim_payload_from_seed x s ss) Htrue_ix Hfalse_ixs Hann_true Hann_false
+      Hshare_true Hshare_false Hglob Hquery Hprog.
+case: (ms3c_phase1_payload_from_public_input x).
+move=> tr fr atr afr str sfr gcr qdr pcr tr0 fr0 atr0 afr0 str0 sfr0 gcr0 qdr0 pcr0 /=.
+move=> Htrue_ix Hfalse_ixs Hann_true Hann_false Hshare_true Hshare_false Hglob Hquery Hprog.
+subst.
+by [].
+qed.
 
 op d_ms3c_real_comparison_payload (x : ms_public_input) : ms3c_real_comparison_payload distr =
   dmap (d_ms3c_real_payload_seed x) (ms3c_real_payload_from_seed x).
@@ -97,9 +208,12 @@ lemma L_ms3c_cross_support_real_sim_payload_equal
   pr = ps.
 proof.
 move=> Hpr Hps.
-case/supp_dmap: Hpr => sr [_ Heqpr].
-case/supp_dmap: Hps => ss [_ Heqps].
-by rewrite Heqpr Heqps /ms3c_real_payload_from_seed /ms3c_sim_payload_from_seed.
+case/supp_dmap: Hpr => sr [Hsr Heqpr].
+case/supp_dmap: Hps => ss [Hss Heqps].
+rewrite Heqpr Heqps.
+have -> := L_ms3c_real_payload_from_seed_on_support_eq_phase1 x sr Hsr.
+have -> := L_ms3c_sim_payload_from_seed_on_support_eq_phase1 x s ss Hss.
+by [].
 qed.
 
 lemma L_ms3c_real_comparison_payload_law_lossless (x : ms_public_input) :
