docs/03-formal-verification/easycrypt/ms/comparison/ComparisonPayloadTypes.ec
@@ -17,11 +17,13 @@ type ms3c_seed_challenge = {
    ms3csc_global_challenge : digest;
    ms3csc_programmed_challenge : digest;
    ms3csc_query_digest : digest;
+   ms3csc_rom_coin : scalar;
 }.
 
 type ms3c_seed_announcement = {
    ms3csa_ann_true : sch_point;
    ms3csa_ann_false : sch_point list;
+   ms3csa_transcript_coin : scalar;
 }.
 
 type ms3c_real_seed_challenge = ms3c_seed_challenge.
@@ -40,7 +42,7 @@ op ms3c_phase1_seed_query_digest (x : ms_public_input) : digest =
    ms_comparison_query_digest (ms3c_public_stmt_digest x)
       (ms3c_phase1_seed_ann_digests x).
 
-op ms3c_phase1_seed_challenge_from_public_input (x : ms_public_input) : ms3c_seed_challenge =
+op ms3c_seed_challenge_with_rom_coin (x : ms_public_input) (rom_coin : scalar) : ms3c_seed_challenge =
    {| ms3csc_stmt_digest = ms3c_public_stmt_digest x;
        ms3csc_true_clause_ix = ms3c_public_true_clause_index x;
        ms3csc_false_clause_ixs = ms3c_public_false_clause_indices x;
@@ -48,11 +50,21 @@ op ms3c_phase1_seed_challenge_from_public_input (x : ms_public_input) : ms3c_see
        ms3csc_share_false = ms3c_public_false_shares x;
        ms3csc_global_challenge = x.`mspi_comparison_global;
        ms3csc_programmed_challenge = x.`mspi_comparison_global;
-       ms3csc_query_digest = ms3c_phase1_seed_query_digest x |}.
+       ms3csc_query_digest = ms3c_phase1_seed_query_digest x;
+       ms3csc_rom_coin = rom_coin |}.
+
+op ms3c_seed_announcement_with_transcript_coin
+   (x : ms_public_input) (transcript_coin : scalar) : ms3c_seed_announcement =
+   {| ms3csa_ann_true = ms3c_public_true_announcement x;
+       ms3csa_ann_false = ms3c_public_false_announcements x;
+       ms3csa_transcript_coin = transcript_coin |}.
+
+op ms3c_phase1_seed_challenge_from_public_input (x : ms_public_input) : ms3c_seed_challenge =
+   ms3c_seed_challenge_with_rom_coin x
+     (ms_query_to_scalar (ms3c_phase1_seed_query_digest x)).
 
 op ms3c_phase1_seed_announcement_from_public_input (x : ms_public_input) : ms3c_seed_announcement =
-   {| ms3csa_ann_true = ms3c_public_true_announcement x;
-       ms3csa_ann_false = ms3c_public_false_announcements x |}.
+   ms3c_seed_announcement_with_transcript_coin x (ms3c_public_true_share x).
 
 op ms3c_phase1_real_payload_seed_from_public_input (x : ms_public_input) : ms3c_real_payload_seed =
    (ms3c_phase1_seed_challenge_from_public_input x,
@@ -80,7 +92,8 @@ lemma L_ms3c_phase1_seed_challenge_uses_public_surface (x : ms_public_input) :
    (ms3c_phase1_seed_challenge_from_public_input x).`ms3csc_query_digest =
       ms3c_phase1_seed_query_digest x.
 proof.
-by rewrite /ms3c_phase1_seed_challenge_from_public_input /=.
+rewrite /ms3c_phase1_seed_challenge_from_public_input.
+by rewrite /ms3c_seed_challenge_with_rom_coin /=.
 qed.
 
 lemma L_ms3c_phase1_seed_announcement_uses_public_surface (x : ms_public_input) :
@@ -89,7 +102,8 @@ lemma L_ms3c_phase1_seed_announcement_uses_public_surface (x : ms_public_input) 
    (ms3c_phase1_seed_announcement_from_public_input x).`ms3csa_ann_false =
       ms3c_public_false_announcements x.
 proof.
-by rewrite /ms3c_phase1_seed_announcement_from_public_input /=.
+rewrite /ms3c_phase1_seed_announcement_from_public_input.
+by rewrite /ms3c_seed_announcement_with_transcript_coin /=.
 qed.
 
 lemma L_ms3c_phase1_real_sim_payload_seed_from_public_input
