docs/03-formal-verification/easycrypt/ms/comparison/ComparisonPayloadSeedAnchors.ec
@@ -16,11 +16,22 @@ pred ms3c_real_from_seed_share_length_anchor
 
 lemma A_ms3c_real_from_seed_uses_share_length :
   forall (x : ms_public_input) (sr : ms3c_real_payload_seed),
+    sr \in d_ms3c_real_payload_seed x =>
     ms3c_real_from_seed_share_length_anchor x sr.
 proof.
-move=> x sr.
+move=> x sr Hsr.
+rewrite /d_ms3c_real_payload_seed supp_dprod in Hsr.
+case: sr Hsr => sc sa /=.
+move=> [Hsc Hsa].
+have [_ [_ [_ [_ [Hshare_false _]]]]] :=
+  L_ms3c_real_seed_challenge_on_support_public_surface x sc Hsc.
+have [_ Hann_false] :=
+  L_ms3c_real_seed_announcement_on_support_public_surface x sa Hsa.
 rewrite /ms3c_real_from_seed_share_length_anchor /ms3c_real_payload_from_seed
-  /ms3c_phase1_payload_from_public_input /=.
+  /ms3c_payload_from_seed_components /= Hshare_false Hann_false.
+rewrite /ms3c_public_false_shares /ms_public_comparison_false_shares.
+rewrite /ms3c_public_false_announcements /ms3c_public_false_openings.
+rewrite /ms_public_comparison_false_openings /ms_public_comparison_false_entries.
 by rewrite !size_map.
 qed.
 
@@ -45,17 +56,23 @@ pred ms3c_real_from_seed_public_index_anchor (x : ms_public_input) (sr : ms3c_re
 
 lemma A_ms3c_real_from_seed_uses_public_indices :
   forall (x : ms_public_input) (sr : ms3c_real_payload_seed),
+    sr \in d_ms3c_real_payload_seed x =>
     ms3c_real_from_seed_public_index_anchor x sr.
 proof.
-move=> x sr.
+move=> x sr Hsr.
+rewrite /d_ms3c_real_payload_seed supp_dprod in Hsr.
+case: sr Hsr => sc sa /=.
+move=> [Hsc Hsa].
+have [_ [Htrue_ix [Hfalse_ixs _]]] :=
+  L_ms3c_real_seed_challenge_on_support_public_surface x sc Hsc.
+have [_ Hann_false] :=
+  L_ms3c_real_seed_announcement_on_support_public_surface x sa Hsa.
 rewrite /ms3c_real_from_seed_public_index_anchor /ms3c_real_payload_from_seed
-  /ms3c_phase1_payload_from_public_input.
+  /ms3c_payload_from_seed_components /=.
 split.
-- by [].
+- exact Hfalse_ixs.
 split.
-- rewrite /ms3c_phase1_comparison_carrier_from_public_input.
-  rewrite /ms3b_phase1_comparison_carrier /ms3c_public_true_clause_index /=.
-  by [].
+- exact Htrue_ix.
 have Hannsz : size (ms3c_public_false_announcements x) =
   size (ms_public_comparison_false_entries x).
   rewrite /ms3c_public_false_announcements /ms3c_public_false_openings.
@@ -66,20 +83,22 @@ have Hixsz : size (ms3c_public_false_clause_indices x) =
   rewrite /ms3c_public_false_clause_indices /ms_public_comparison_false_indices.
   rewrite /ms_public_comparison_false_entries.
   by rewrite size_map.
-by rewrite Hannsz Hixsz.
+by rewrite Hann_false Hfalse_ixs Hannsz Hixsz.
 qed.
 
 lemma L_ms3c_real_seed_index_shape_valid (x : ms_public_input) (sr : ms3c_real_payload_seed) :
-  ms3c_real_from_seed_public_index_anchor x sr =>
+  sr \in d_ms3c_real_payload_seed x =>
   0 <= (ms3c_real_payload_from_seed x sr).`mscp_true_clause_ix /\
   size (ms3c_real_payload_from_seed x sr).`mscp_ann_false =
   size (ms3c_real_payload_from_seed x sr).`mscp_false_clause_ixs.
 proof.
-move=> [Hfalse_ixs [Htrue_ix Hsz_ann_false]].
+move=> Hsr.
+have [Hfalse_ixs [Htrue_ix Hsz_ann_false]] :=
+  A_ms3c_real_from_seed_uses_public_indices x sr Hsr.
 split.
 - have [Hix _] := L_ms3c_public_shape_ok_of_native_slice x.
-  rewrite /ms3c_real_payload_from_seed /ms3c_phase1_payload_from_public_input.
-  rewrite /ms3c_phase1_comparison_carrier_from_public_input /ms3b_phase1_comparison_carrier /=.
+  have -> : (ms3c_real_payload_from_seed x sr).`mscp_true_clause_ix =
+      ms3c_public_true_clause_index x by exact Htrue_ix.
   exact Hix.
 by exact Hsz_ann_false.
 qed.
@@ -91,11 +110,22 @@ pred ms3c_sim_from_seed_share_length_anchor
 
 lemma A_ms3c_sim_from_seed_uses_share_length :
   forall (x : ms_public_input) (s : seed) (ss : ms3c_sim_payload_seed),
+    ss \in d_ms3c_sim_payload_seed x s =>
     ms3c_sim_from_seed_share_length_anchor x s ss.
 proof.
-move=> x s ss.
+move=> x s ss Hss.
+rewrite /d_ms3c_sim_payload_seed supp_dprod in Hss.
+case: ss Hss => sc sa /=.
+move=> [Hsc Hsa].
+have [_ [_ [_ [_ [Hshare_false _]]]]] :=
+  L_ms3c_sim_seed_challenge_on_support_public_surface x s sc Hsc.
+have [_ Hann_false] :=
+  L_ms3c_sim_seed_announcement_on_support_public_surface x s sa Hsa.
 rewrite /ms3c_sim_from_seed_share_length_anchor /ms3c_sim_payload_from_seed
-  /ms3c_phase1_payload_from_public_input /=.
+  /ms3c_payload_from_seed_components /= Hshare_false Hann_false.
+rewrite /ms3c_public_false_shares /ms_public_comparison_false_shares.
+rewrite /ms3c_public_false_announcements /ms3c_public_false_openings.
+rewrite /ms_public_comparison_false_openings /ms_public_comparison_false_entries.
 by rewrite !size_map.
 qed.
 
@@ -122,17 +152,23 @@ pred ms3c_sim_from_seed_public_index_anchor
 
 lemma A_ms3c_sim_from_seed_uses_public_indices :
   forall (x : ms_public_input) (s : seed) (ss : ms3c_sim_payload_seed),
+    ss \in d_ms3c_sim_payload_seed x s =>
     ms3c_sim_from_seed_public_index_anchor x s ss.
 proof.
-move=> x s ss.
+move=> x s ss Hss.
+rewrite /d_ms3c_sim_payload_seed supp_dprod in Hss.
+case: ss Hss => sc sa /=.
+move=> [Hsc Hsa].
+have [_ [Htrue_ix [Hfalse_ixs _]]] :=
+  L_ms3c_sim_seed_challenge_on_support_public_surface x s sc Hsc.
+have [_ Hann_false] :=
+  L_ms3c_sim_seed_announcement_on_support_public_surface x s sa Hsa.
 rewrite /ms3c_sim_from_seed_public_index_anchor /ms3c_sim_payload_from_seed
-  /ms3c_phase1_payload_from_public_input.
+  /ms3c_payload_from_seed_components /=.
 split.
-- by [].
+- exact Hfalse_ixs.
 split.
-- rewrite /ms3c_phase1_comparison_carrier_from_public_input.
-  rewrite /ms3b_phase1_comparison_carrier /ms3c_public_true_clause_index /=.
-  by [].
+- exact Htrue_ix.
 have Hannsz : size (ms3c_public_false_announcements x) =
   size (ms_public_comparison_false_entries x).
   rewrite /ms3c_public_false_announcements /ms3c_public_false_openings.
@@ -143,21 +179,23 @@ have Hixsz : size (ms3c_public_false_clause_indices x) =
   rewrite /ms3c_public_false_clause_indices /ms_public_comparison_false_indices.
   rewrite /ms_public_comparison_false_entries.
   by rewrite size_map.
-by rewrite Hannsz Hixsz.
+by rewrite Hann_false Hfalse_ixs Hannsz Hixsz.
 qed.
 
 lemma L_ms3c_sim_seed_index_shape_valid
   (x : ms_public_input) (s : seed) (ss : ms3c_sim_payload_seed) :
-  ms3c_sim_from_seed_public_index_anchor x s ss =>
+  ss \in d_ms3c_sim_payload_seed x s =>
   0 <= (ms3c_sim_payload_from_seed x s ss).`mscp_true_clause_ix /\
   size (ms3c_sim_payload_from_seed x s ss).`mscp_ann_false =
   size (ms3c_sim_payload_from_seed x s ss).`mscp_false_clause_ixs.
 proof.
-move=> [Hfalse_ixs [Htrue_ix Hsz_ann_false]].
+move=> Hss.
+have [Hfalse_ixs [Htrue_ix Hsz_ann_false]] :=
+  A_ms3c_sim_from_seed_uses_public_indices x s ss Hss.
 split.
 - have [Hix _] := L_ms3c_public_shape_ok_of_native_slice x.
-  rewrite /ms3c_sim_payload_from_seed /ms3c_phase1_payload_from_public_input.
-  rewrite /ms3c_phase1_comparison_carrier_from_public_input /ms3b_phase1_comparison_carrier /=.
+  have -> : (ms3c_sim_payload_from_seed x s ss).`mscp_true_clause_ix =
+      ms3c_public_true_clause_index x by exact Htrue_ix.
   exact Hix.
 by exact Hsz_ann_false.
 qed.
